\section{Reglas de derivación}
\begin{center}
$ (f+g)'(x) = f'(a)+g'(a) \hspace{1cm}
(fg)'(x) = f'(a)g(a) + f(a)g'(a) \hspace{1cm}
\left(\frac{f}{g}\right)'(a) = \frac{f'(a)g(a) - f(a)g'(a)}{g(a)^2}$
\end{center}
\subsection{Regla de la cadena}
$f:A\rightarrow\R$, $g:B\rightarrow\R$ con $f(A)\subset B$ y $a\in A\cap A'$, deben ser $f$ derivable en $a$ y $g$ derivable en $f(a)$
$$ (gof)'(a) = g'(f(a))f'(a) $$
Sea una función $f:A\rightarrow\R$ inyectiva con inversa derivable en $a$, entonces $f(a)\in f(A)$, son equivalentes
\begin{itemize}
	\item $f'(a)\not =0$ y $f^{-1}$ es continua en $f(a)$
	\item $f^{-1}$ es derivable en $f(a)$
\end{itemize}
$$ (f^{-1})'(f(a)) = \frac{1}{f'(a)} $$
$$ f'(x^k) = kx^{k-1} \ \ k\in\N \hspace{1.5cm}
 f'(\sqrt[q]{x}) = \frac{1}{ q(\sqrt[q]{x})^{q-1} }$$
